\documentclass[10pt,a5paper]{article}
\usepackage[margin=.8cm]{geometry}
\usepackage[utf8]{inputenc}
\usepackage[IL2]{fontenc}
\usepackage[czech]{babel}
\usepackage{microtype}
\usepackage{amssymb}
\usepackage{amsthm}
\usepackage{amsmath}
\usepackage{xcolor}
\usepackage{graphicx}
\usepackage{wasysym}
\usepackage{multicol}

\usepackage[inline]{enumitem}

\newcommand{\R}{\mathbb{R}}

\newcommand{\hint}[1]{{\color{gray}\footnotesize\noindent(Nápověda: #1)}}

\setlist[enumerate]{label={\textbf{\arabic*.}},topsep=\smallskipamount,itemsep=1\medskipamount,parsep=0pt,itemjoin={\quad}}
\setlist[itemize]{topsep=\smallskipamount,noitemsep}

\def\tisk{%
\newbox\shipouthackbox
\pdfpagewidth=2\pdfpagewidth
\let\oldshipout=\shipout
\def\shipout{\afterassignment\zdvojtmp \setbox\shipouthackbox=}%
\def\zdvojtmp{\aftergroup\zdvoj}%
\def\zdvoj{%
    \oldshipout\vbox{\hbox{%
        \copy\shipouthackbox
        \hskip\dimexpr .5\pdfpagewidth-\wd\shipouthackbox\relax
        \box\shipouthackbox
    }}%
}}%



\newtheorem*{poz}{Pozorování}

\theoremstyle{definition}
\newtheorem{uloha}{\atr Úloha}
\newtheorem{suloha}[uloha]{\llap{$\star$ }Úloha}
\newtheorem*{bonus}{Bonus}
\newtheorem*{defn}{Definice}

\pagestyle{empty}

\let\ee\expandafter

\def\vysld{}
\let\printvysl\relax
\let\printalphvysl\relax

\def\substd{}

\makeatletter
\long\def\vysl#1{\ee\ee\ee\gdef\ee\ee\ee\vysld\ee\ee\ee{\ee\vysld\ee\printvysl\ee{\the\c@uloha}{#1}}}
\let\vyslplain\vysl

\def\locvysl#1{\ee\gdef\ee\locvysld\ee{\locvysld\item #1}}
\let\lv\locvysl

\long\def\itvysl#1{\ee\gdef\ee\vysld\ee{\vysld\printvysl{#1}}}
\long\def\itsubst#1{\ee\gdef\ee\substd\ee{\substd\printsubst{#1}}}
\def\pr#1#2#3{\item $#1$\itvysl{#2}\itsubst{#3}}
\def\pri#1#2#3{\stitem $#1$\itvysl{#2}\itsubst{#3}}
\def\prii#1#2#3{\ststitem $#1$\itvysl{#2}\itsubst{#3}}

\newenvironment{ulohav}[1][]{\begin{uloha}[#1]\gdef\locvysld{\begin{enumerate*}}}{\ee\vyslplain\ee{\locvysld\end{enumerate*}}\end{uloha}}
%

\def\stitem{\@noitemargtrue\@item[$\star$ \@itemlabel]}
\def\ststitem{\@noitemargtrue\@item[$\star\star$ \@itemlabel]}

\makeatother

\def\atr{}
\def\basic{\def\atr{\llap{\mdseries$\sun$ }\gdef\atr{}}}
\def\interest{\def\atr{\llap{$\star$ }\gdef\atr{}}}
\let\mb\mathbf

\let\la\langle
\let\ra\rangle
\def\bla{\bigl\la}
\def\bra{\bigr\ra}
\def\blz{\bigl(}
\def\brz{\bigr)}

\def\R{\mathbb{R}}
\def\N{\mathbb{N}}

\let\results\newpage
\let\endresults\relax

\def\resultssame{%
    \long\def\results##1\endresults{%
        \vfill\noindent\rotatebox{180}{\vbox{##1}}%
    }%
}

\begin{document}

%\resultssame
%\tisk


\begin{center}
    \textbf{\LARGE (Přímočará) sbírka}\\[1mm]
    na\\[1mm]
    {\Large substituci v rovnicích, nerovnicích a jejich soustavách}
\end{center}


\begin{multicols}{2}
\everymath{\displaystyle}
\begin{enumerate}[itemsep=\bigskipamount]
    \rightskip=0pt plus1fil\relax
    \lineskip=4pt\relax
    \pr{4x^4 - x^2 - 18 = 0}{\{\pm\frac32\}}{x^2}
    \pr{(|x|-2)(|x|-3)(|x|+4) = 0}{\{\pm2; \pm3\}}{|x|}
    \pr{\left|\frac1x + 1\right| = \frac2x - 1}{\{\frac12\}}{\frac1x}
    \pr{(x^2+2x-3)(x^2 + 2x+1)-5 = 0}{\{-1\pm\sqrt5\}}{x^2 + 2x}
    \pr{\frac{(x^2-2x+8)^2}{(x^2 - 2x)^2}=4}{\{-2;4\}}{x^2 - 2x}
    \pr{x^2 + |x| - \frac{3}{x^2 + |x| + 1} = 1}{\{\pm1\}}{x^2 + |x|}
    \pr{\left(\frac{x^2+2}{x^2-4}-3\right)\left(\frac{x^2+2}{x^2-4}+4\right)=-10}{\{\pm\sqrt2\}}{\frac{x^2+2}{x^2-4}}
    \pr{|x^2 + 5x| - 2\cdot |x^2 + 5x - 3| + 8 = 0}{\{-7; 2; \frac12(-5\pm\sqrt{17})\}}{x^2 + 5x}
    \pr{(x^4 + 2 x^2)^2 - 7 (x^4 + 2 x^2) + 12 = 0}{\{\pm1; \pm\sqrt{\sqrt5-1}\}}{\text{nejprve }x^4+2x^2,\text{ pak }x^2}
    \pri{\Bigl|\bigl||x|-1\bigr|-1\Bigr| = 1}{\{-3;-1;1;3\}}{\text{nejprve }\bigl||x|-1\bigr|,\text{ pak }|x|}
    \prii{2x^3 - 3x^2 - 3x + 2 = 0}{\{-1; 2; \frac12\}}{x + \frac1x}
    \pr{\frac1x + \frac3y = 5,\quad \frac2x-\frac6y = 6}{\{[\frac14; 3]\}}{\frac1x, \frac3y}
    \pr{\frac{2}{x+y}-\frac{5}{x-y}=1$, $\frac{1}{x+y}+\frac{4}{x-y}=\frac95}{\{[3;-2]\}}{\frac{1}{x+y}, \frac{1}{x-y}}
    \pr{\frac{x+1}{x+y} + \frac{y}{x-y}=\frac32$, $2 \cdot \frac{x+1}{x+y} - 3\cdot \frac{y}{x-y}=\frac12}{\{[3;1]\}}{\frac{x+1}{x+y}, \frac{y}{x-y}}
    \pr{x^2 + 2y^2 = 7$,\quad $2x^2 + 3y^2 = 11}{\{[-1;-\sqrt3]; [-1;\sqrt3]; [1;-\sqrt3]; [1;\sqrt3]\}}{x^2, y^2}
    \pr{|x+2|+2|y-3|=15$, $|x+2| - 4|y-3|=3}{\{[-13;1]; [9;1]; [-13;5]; [9;5]\}}{|x+2|, |y-3|}
    \pri{x^4-5 x^2+6\geq 0}{(-\infty;-\sqrt3\rangle \cup \langle-\sqrt2;\sqrt2\rangle \cup \langle\sqrt3; \infty)}{x^2}
    \pri{x^4+5 x^2+6\geq 0}{\R}{x^2}
    \pri{\left(\frac{x+1}{2x+3}-1\right)\left(\frac{x+1}{2x+3}-2\right)\geq0}{(-\infty;-2\rangle\cup \langle-\frac53;-\frac32)\cup(-\frac32;\infty)}{\frac{x+1}{2x+3}}
\end{enumerate}
\end{multicols}


\results

\subsection*{Substituce}
Mohou samozřejmě fungovat i jiné než tyto volby.
\begin{multicols}{2}
\def\printsubst#1{\item $#1$}
\begin{enumerate}
    \substd
\end{enumerate}
\end{multicols}


\subsection*{Výsledky}
\begin{multicols}{2}
\def\printvysl#1{\item $#1$}
\begin{enumerate}
    \vysld
\end{enumerate}
\end{multicols}
\endresults


\end{document}